chapter04/solutions/leader_election_nosafety.dfy
@@ -8,21 +8,23 @@ predicate ValidIdx(k: Constants, i: nat) {
   0<=i<|k.ids|
 }
 
-predicate UniqueIds(k: Constants) {
-  (forall i, j | ValidIdx(k, i) && ValidIdx(k, j) && k.ids[i]==k.ids[j] :: i == j)
+predicate UniqueIDs(k: Constants) {
+  // No two nodes have the same identifier.
+  && (forall i:nat, j:nat | ValidIdx(k, i) && ValidIdx(k, j) && k.ids[i]==k.ids[j]
+    :: i == j)
 }
 
 predicate WF(k: Constants, s: Variables) {
   && 0 < |k.ids|
-  && UniqueIds(k)
   && |s.highest_heard| == |k.ids|
+  && UniqueIDs(k)
 }
 
 predicate Init(k: Constants, s: Variables)
 {
   && WF(k, s)
     // Everyone begins having heard about nobody, not even themselves.
-  && (forall i | ValidIdx(k, i) :: s.highest_heard[i] == -1)
+  && (forall i:nat | ValidIdx(k, i) :: s.highest_heard[i] == -1)
 }
 
 function max(a: nat, b: nat) : nat {
@@ -43,16 +45,11 @@ predicate Transmission(k: Constants, s: Variables, s': Variables, src: nat)
   && 0 <= src < |k.ids|
 
   // Neighbor address in ring.
-  // TODO let's try it with modulo, too.
   && var dst := NextIdx(k, src);
-  // Yeah turns out modulo makes dafny stupid.
-  // && var dst := (src + 1) % |k.ids|;
 
   // src sends the max of its highest_heard value and its own id.
   && var message := max(s.highest_heard[src], k.ids[src]);
   && var dst_new_max := max(s.highest_heard[dst], message);
-  // Here's bug 1: we compute the max of the message with the highest_heard of dst,
-  // and then ignore it.
 
   && s' == s.(highest_heard := s.highest_heard[dst := dst_new_max])
 }
@@ -78,43 +75,34 @@ predicate IsLeader(k: Constants, s: Variables, i: nat)
   && s.highest_heard[i] == k.ids[i]
 }
 
-// TODO note that the elected leader isn't stable, which isn't ideal.
 predicate Safety(k: Constants, s: Variables)
   requires WF(k, s)
 {
   forall i, j | IsLeader(k, s, i) && IsLeader(k, s, j) :: i == j
 }
 
-predicate IsMaxId(k: Constants, i: nat)
-  requires ValidIdx(k, i)
+predicate IsMaxId(k: Constants, id: nat)
 {
-  forall j | ValidIdx(k, j) :: k.ids[j] <= k.ids[i]
+  forall j:nat | ValidIdx(k, j) :: k.ids[j] <= id
 }
 
-predicate Between(k: Constants, startExclusive: nat, idx: nat, endExclusive: nat)
-  requires ValidIdx(k, startExclusive)
-  requires ValidIdx(k, idx)
-  requires ValidIdx(k, endExclusive)
-{
-  if startExclusive < endExclusive
-  then startExclusive < idx < endExclusive
-  else idx < endExclusive || startExclusive < idx
-}
-
-// An identifier that has "reached" a distant node some way around the
-// ring is at least as high as the id of every node it has passed.
-predicate IDOnChordDominatesIDs(k: Constants, s: Variables)
+predicate InvPred(k: Constants, s: Variables)
   requires WF(k, s)
 {
-  forall i, j | ValidIdx(k, i) && ValidIdx(k, j) && k.ids[i] == s.highest_heard[j] ::
-    forall m | ValidIdx(k, m) && Between(k, i, m, j) :: k.ids[i] > k.ids[m]
+  forall i:nat | ValidIdx(k, i) && !IsMaxId(k, k.ids[i]) :: !IsLeader(k, s, i)
+}
+
+predicate HighestHeardDominatesID(k: Constants, s: Variables)
+  requires WF(k, s)
+{
+  forall i:nat | ValidIdx(k, i) && s.highest_heard[i] != -1 :: s.highest_heard[i] >= k.ids[i]
 }
 
 predicate Inv(k: Constants, s: Variables)
 {
   && WF(k, s)
-  && Safety(k, s)
-  && IDOnChordDominatesIDs(k, s)
+  && InvPred(k, s)
+  && HighestHeardDominatesID(k, s)
 }
 
 lemma InitImpliesInv(k: Constants, s: Variables)
